thys/MFODL_Monitor_Devel/Typing.thy
@@ -1,0 +1,253 @@
+(*<*)
+theory Typing
+  imports Formula
+begin
+(*>*)
+
+section \<open>Typing\<close>
+
+subsection \<open>Types and type classes\<close>
+
+datatype ty = TInt | TFloat | TString
+
+fun ty_of :: "event_data \<Rightarrow> ty" where
+  "ty_of (EInt _) = TInt"
+| "ty_of (EFloat _) = TFloat"
+| "ty_of (EString _) = TString"
+
+definition "numeric_ty = {TInt, TFloat}"
+
+
+subsection \<open>Terms\<close>
+
+type_synonym tyenv = "nat \<Rightarrow> ty"
+
+inductive wty_trm :: "tyenv \<Rightarrow> Formula.trm \<Rightarrow> ty \<Rightarrow> bool" ("(_)/ \<turnstile> (_) :: _" [50,50,50] 50)
+  for E where
+  Var: "E x = t \<Longrightarrow> E \<turnstile> Formula.Var x :: t"
+| Const: "ty_of x = t \<Longrightarrow> E \<turnstile> Formula.Const x :: t"
+| Plus: "E \<turnstile> x :: t \<Longrightarrow> E \<turnstile> y :: t \<Longrightarrow> t \<in> numeric_ty \<Longrightarrow> E \<turnstile> Formula.Plus x y :: t"
+(* TODO: remaining cases *)
+
+lemma ty_of_plus: "ty_of x = t \<Longrightarrow> ty_of y = t \<Longrightarrow> t \<in> numeric_ty \<Longrightarrow> ty_of (x + y) = t"
+  by (cases x; cases y) (simp_all add: numeric_ty_def)
+
+lemma ty_of_eval_trm: "E \<turnstile> x :: t \<Longrightarrow> \<forall>y\<in>fv_trm x. y < length v \<and> ty_of (v ! y) = E y \<Longrightarrow>
+  ty_of (Formula.eval_trm v x) = t"
+  by (induction pred: wty_trm) (simp_all add: ty_of_plus)
+
+lemma wty_trm_fv_cong:
+  assumes "\<And>y. y \<in> fv_trm x \<Longrightarrow> E y = E' y"
+  shows "E \<turnstile> x :: t \<longleftrightarrow> E' \<turnstile> x :: t"
+proof -
+  have "E \<turnstile> x :: t \<Longrightarrow> (\<And>y. y \<in> fv_trm x \<Longrightarrow> E y = E' y) \<Longrightarrow> E' \<turnstile> x :: t" for E E'
+    by (induction pred: wty_trm) (auto intro: wty_trm.intros)
+  with assms show ?thesis by auto
+qed
+
+
+subsection \<open>Formulas\<close>
+
+type_synonym sig = "Formula.name \<rightharpoonup> ty list"
+
+definition wty_tuple :: "ty list \<Rightarrow> event_data list \<Rightarrow> bool" where
+  "wty_tuple = list_all2 (\<lambda>t x. ty_of x = t)"
+
+definition wty_event :: "sig \<Rightarrow> Formula.name \<Rightarrow> event_data list \<Rightarrow> bool" where
+  "wty_event S p xs \<longleftrightarrow> (case S p of Some ts \<Rightarrow> wty_tuple ts xs | None \<Rightarrow> True)"
+
+definition wty_envs :: "sig \<Rightarrow> Formula.trace \<Rightarrow> (Formula.name \<rightharpoonup> nat \<Rightarrow> event_data list set) \<Rightarrow> bool" where
+  "wty_envs S \<sigma> V \<longleftrightarrow> (\<forall>i.
+    (\<forall>(p,xs)\<in>\<Gamma> \<sigma> i. p \<notin> dom V \<longrightarrow> wty_event S p xs) \<and>
+    (\<forall>p\<in>dom V. \<forall>xs\<in>the (V p) i. wty_event S p xs))"
+
+abbreviation wty_trace :: "sig \<Rightarrow> Formula.trace \<Rightarrow> bool" where
+  "wty_trace S \<sigma> \<equiv> wty_envs S \<sigma> Map.empty"
+
+definition wty_db :: "sig \<Rightarrow> (Formula.name \<times> event_data list) set \<Rightarrow> bool" where
+  "wty_db S db \<longleftrightarrow> (\<forall>(p, xs) \<in> db. wty_event S p xs)"
+
+lift_definition wty_prefix :: "sig \<Rightarrow> Formula.prefix \<Rightarrow> bool" is
+  "\<lambda>S \<pi>. \<forall>x\<in>set \<pi>. wty_db S (fst x)" .
+
+lemma wty_pnil: "wty_prefix S pnil"
+  by (transfer fixing: S) simp
+
+lemma wty_psnoc: "wty_prefix S \<pi> \<Longrightarrow> wty_db S (fst x) \<Longrightarrow> last_ts \<pi> \<le> snd x \<Longrightarrow>
+  wty_prefix S (psnoc \<pi> x)"
+  by (transfer fixing: S x) simp
+
+lemma wty_envs_\<Gamma>_D: "wty_envs S \<sigma> V \<Longrightarrow> p \<notin> dom V \<Longrightarrow> (p, xs) \<in> \<Gamma> \<sigma> i \<Longrightarrow> S p = Some ts \<Longrightarrow>
+  wty_tuple ts xs"
+  by (fastforce simp: wty_envs_def wty_event_def split: option.splits)
+
+lemma wty_envs_V_D: "wty_envs S \<sigma> V \<Longrightarrow> p \<in> dom V \<Longrightarrow> xs \<in> the (V p) i \<Longrightarrow> S p = Some ts \<Longrightarrow>
+  wty_tuple ts xs"
+  by (fastforce simp: wty_envs_def wty_event_def split: option.splits)
+
+inductive wty_formula :: "sig \<Rightarrow> tyenv \<Rightarrow> Formula.formula \<Rightarrow> bool" ("(_),/ (_)/ \<turnstile> (_)" [50,50,50] 50) where
+  Pred: "S p = Some tys \<Longrightarrow> list_all2 (\<lambda>tm ty. E \<turnstile> tm :: ty) tms tys \<Longrightarrow> S, E \<turnstile> Formula.Pred p tms"
+| Let: "S, E' \<turnstile> \<phi> \<Longrightarrow> S(p \<mapsto> tabulate E' 0 (Formula.nfv \<phi>)), E \<turnstile> \<psi> \<Longrightarrow> S, E \<turnstile> Formula.Let p \<phi> \<psi>"
+| And: "S, E \<turnstile> \<phi> \<Longrightarrow> S, E \<turnstile> \<psi> \<Longrightarrow> S, E \<turnstile> Formula.And \<phi> \<psi>"
+| Exists: "S, case_nat t E \<turnstile> \<phi> \<Longrightarrow> S, E \<turnstile> Formula.Exists \<phi>"
+(* TODO: remaining cases *)
+
+lemma wty_formula_fv_cong:
+  assumes "\<And>y. y \<in> fv \<phi> \<Longrightarrow> E y = E' y"
+  shows "S, E \<turnstile> \<phi> \<longleftrightarrow> S, E' \<turnstile> \<phi>"
+proof -
+  have "S, E \<turnstile> \<phi> \<Longrightarrow> (\<And>y. y \<in> fv \<phi> \<Longrightarrow> E y = E' y) \<Longrightarrow> S, E' \<turnstile> \<phi>" for E E'
+  proof (induction arbitrary: E' pred: wty_formula)
+    case (Pred S p tys E tms)
+    then show ?case
+      by (fastforce intro!: wty_formula.Pred
+          elim!: list.rel_mono_strong wty_trm_fv_cong[THEN iffD1, rotated])
+  next
+    case (Exists S t E \<phi>)
+    then show ?case
+      by (fastforce simp: fvi_Suc intro!: wty_formula.Exists[where t=t] split: nat.split)
+  qed (auto intro: wty_formula.intros)
+  with assms show ?thesis by auto
+qed
+
+lemma ty_of_sat_safe: "safe_formula \<phi> \<Longrightarrow> S, E \<turnstile> \<phi> \<Longrightarrow> wty_envs S \<sigma> V \<Longrightarrow>
+  Formula.sat \<sigma> V v i \<phi> \<Longrightarrow> x \<in> Formula.fv \<phi> \<Longrightarrow> x < length v \<Longrightarrow> ty_of (v ! x) = E x"
+proof (induction arbitrary: S E V v i x rule: safe_formula_induct)
+  case (Eq_Const c d)
+  then show ?case by cases (* TODO *)
+next
+  case (Eq_Var1 c x)
+  then show ?case by cases (* TODO *)
+next
+  case (Eq_Var2 c x)
+  then show ?case by cases (* TODO *)
+next
+  case (neq_Var x)
+  then show ?case by cases (* TODO *)
+next
+  case (Pred p tms)
+  from Pred.prems(1) obtain tys where
+    S_p: "S p = Some tys" and
+    xs_ts: "list_all2 (\<lambda>tm ty. E \<turnstile> tm :: ty) tms tys"
+    by cases
+  let ?xs = "map (Formula.eval_trm v) tms"
+  have wty_xs: "wty_tuple tys ?xs"
+  proof (cases "p \<in> dom V")
+    case True
+    then have "?xs \<in> the (V p) i"
+      using Pred.prems(3) by auto
+    with True show ?thesis
+      using Pred.prems(2) by (auto simp: S_p dest!: wty_envs_V_D)
+  next
+    case False
+    then have "(p, ?xs) \<in> \<Gamma> \<sigma> i"
+      using Pred.prems(3) by (auto split: option.splits)
+    with False show ?thesis
+      using Pred.prems(2) by (auto simp: S_p dest!: wty_envs_\<Gamma>_D)
+  qed
+  from Pred obtain k where k: "k < length tms" "tms ! k = Formula.Var x"
+    by (fastforce simp: trm.is_Var_def trm.is_Const_def in_set_conv_nth)
+  with Pred.prems have "v ! x = ?xs ! k" by simp
+  with wty_xs k have "ty_of (v ! x) = tys ! k"
+    by (auto simp: wty_tuple_def list_all2_conv_all_nth)
+  also have "\<dots> = E x"
+    using xs_ts k
+    by (fastforce simp: list_all2_conv_all_nth elim: wty_trm.cases)
+  finally show ?case .
+next
+  case (Let p \<phi> \<psi>)
+  let ?V' = "V(p \<mapsto> \<lambda>i. {v. length v = Formula.nfv \<phi> \<and> Formula.sat \<sigma> V v i \<phi>})"
+  from Let.prems(1) obtain E' where
+    wty_\<phi>: "S, E' \<turnstile> \<phi>" and
+    wty_\<psi>: "S(p \<mapsto> tabulate E' 0 (Formula.nfv \<phi>)), E \<turnstile> \<psi>"
+    by (cases pred: wty_formula)
+  let ?tys = "tabulate E' 0 (Formula.nfv \<phi>)"
+  {
+    fix v' i
+    assume "length v' = Formula.nfv \<phi>" and "Formula.sat \<sigma> V v' i \<phi>"
+    then have "wty_tuple ?tys v'"
+      using Let.IH(1) wty_\<phi> Let.prems(2) Let.hyps(1)
+      by (auto simp: wty_tuple_def list_all2_conv_all_nth)
+  }
+  with Let.prems(2) have "wty_envs (S(p \<mapsto> ?tys)) \<sigma> ?V'"
+    by (auto simp: wty_envs_def wty_event_def)
+  from Let.prems(3) have "Formula.sat \<sigma> ?V' v i \<psi>" by simp
+  from Let.prems(4) have "x \<in> fv \<psi>" by simp
+  show ?case by (rule Let.IH(2)) fact+
+next
+  case (And_assign \<phi> \<psi>) (* TODO *)
+  from And_assign.hyps(2) obtain a b where \<psi>_eq: "\<psi> = Formula.Eq a b"
+    by (auto simp: safe_assignment_def split: formula.splits)
+  from And_assign.prems(1) show ?case
+    unfolding \<psi>_eq by (blast elim: wty_formula.cases)
+next
+  case (And_safe \<phi> \<psi>)
+  from And_safe.prems(1) obtain "S, E \<turnstile> \<phi>" and "S, E \<turnstile> \<psi>" by cases
+  from And_safe.prems(3) have "Formula.sat \<sigma> V v i \<phi>" and "Formula.sat \<sigma> V v i \<psi>"
+    by simp_all
+  from And_safe.prems(4) consider (in_\<phi>) "x \<in> fv \<phi>" | (in_\<psi>) "x \<in> fv \<psi>" by auto
+  then show ?case
+  proof cases
+    case in_\<phi>
+    show ?thesis by (rule And_safe.IH(1)) fact+
+  next
+    case in_\<psi>
+    show ?thesis by (rule And_safe.IH(2)) fact+
+  qed
+next
+  case (And_constraint \<phi> \<psi>) (* TODO *)
+  from \<open>is_constraint \<psi>\<close> show ?case
+    by (cases \<psi> rule: is_constraint.cases)
+      (use And_constraint.prems(1) in "auto elim: wty_formula.cases")
+next
+  case (And_Not \<phi> \<psi>)
+  then show ?case by (blast elim: wty_formula.cases) (* TODO *)
+next
+  case (Ands l pos neg)
+  from Ands.prems(1) show ?case by cases (* TODO *)
+next
+  case (Neg \<phi>)
+  from Neg.prems(1) show ?case by cases (* TODO *)
+next
+  case (Or \<phi> \<psi>)
+  from Or.prems(1) show ?case by cases (* TODO *)
+next
+  case (Exists \<phi>)
+  from Exists.prems(1) obtain t where "S, case_nat t E \<turnstile> \<phi>" by cases
+  from Exists.prems(3) obtain z where "Formula.sat \<sigma> V (z#v) i \<phi>" by auto
+  from Exists.prems(4) have "Suc x \<in> fv \<phi>" by (simp add: fvi_Suc)
+  have "ty_of ((z#v) ! Suc x) = case_nat t E (Suc x)"
+    by (rule Exists.IH) (simp?, fact)+
+  then show ?case by simp
+next
+  case (Agg y \<omega> b f \<phi>)
+  from Agg.prems(1) show ?case by cases (* TODO *)
+next
+  case (Prev I \<phi>)
+  from Prev.prems(1) show ?case by cases (* TODO *)
+next
+  case (Next I \<phi>)
+  from Next.prems(1) show ?case by cases (* TODO *)
+next
+  case (Since \<phi> I \<psi>)
+  from Since.prems(1) show ?case by cases (* TODO *)
+next
+  case (Not_Since \<phi> I \<psi>)
+  from Not_Since.prems(1) show ?case by cases (* TODO *)
+next
+  case (Until \<phi> I \<psi>)
+  from Until.prems(1) show ?case by cases (* TODO *)
+next
+  case (Not_Until \<phi> I \<psi>)
+  from Not_Until.prems(1) show ?case by cases (* TODO *)
+next
+  case (MatchP I r)
+  from MatchP.prems(1) show ?case by cases (* TODO *)
+next
+  case (MatchF I r)
+  from MatchF.prems(1) show ?case by cases (* TODO *)
+qed
+
+(*<*)
+end
+(*>*)
